Logic/Propositional/Superintuitionistic/Kripke/LEM.lean
@@ -1,0 +1,36 @@
+import Logic.Propositional.Superintuitionistic.Kripke.Semantics
+
+/-!
+  # Counterexamples to the Law of Excluded Middle in Intuitionistic Logic
+
+  ## Theorems
+  - `noLEM`: LEM is not always valid in intuitionistic logic.
+-/
+
+namespace LO.Propositional.Superintuitionistic.Kripke
+
+def LEMCounterexampleModel : Model (𝐈𝐧𝐭 (Fin 2) α) where
+  frame := λ w₁ w₂ => (w₁ = w₂) ∨ (w₁ = 0)
+  valuation w _ := w = 1;
+  hereditary := by simp; aesop;
+  frame_prop := by
+    simp [FrameClass.Intuitionistic];
+    constructor;
+    . simp [Transitive]; aesop;
+    . simp [Reflexive];
+
+open Formula Formula.Kripke
+
+lemma noLEM_atom {a : α} : ¬(LEMCounterexampleModel ⊧ (atom a) ⋎ ~(atom a)) := by
+  simp [ValidOnModel.iff_models, Satisfies.iff_models, ValidOnModel, Satisfies, LEMCounterexampleModel];
+  existsi 0;
+  simp_all;
+
+variable [Inhabited α]
+
+theorem noLEM : ¬(∀ p, (𝐈𝐧𝐭 (Fin 2) α) ⊧ p ⋎ ~p) := by
+  simp [ValidOnFrameClass.iff_models, ValidOnFrameClass];
+  existsi (atom default), LEMCounterexampleModel;
+  apply noLEM_atom
+
+end LO.Propositional.Superintuitionistic.Kripke
