Logic/Propositional/Superintuitionistic/Kripke/Soundness.lean
@@ -1,0 +1,29 @@
+import Logic.Propositional.Superintuitionistic.Deduction
+import Logic.Propositional.Superintuitionistic.Kripke.Semantics
+
+namespace LO.Propositional.Superintuitionistic.Kripke
+
+variable {W α : Type*}
+
+open Formula.Kripke.ValidOnFrameClass
+
+-- TODO: Expand 𝐄𝐅𝐐-𝐈𝐧𝐭
+
+lemma sound (d : 𝐄𝐅𝐐 ⊢ p) : (𝐈𝐧𝐭 W α) ⊧ p := by
+  induction d with
+  | eaxm h =>
+    obtain ⟨q, hq⟩ := by simpa [axiomEFQ] using h;
+    subst hq;
+    simp;
+  | mdp _ _ ihpq ihp => exact mdp (by simp_all) ihpq ihp;
+  | conj₃ => apply conj₃; simp_all;
+  | disj₃ => apply disj₃; simp_all;
+  | imply₁ => apply imply₁; simp_all;
+  | imply₂ => apply imply₂; simp_all; simp_all;
+  | _ => simp_all;
+
+lemma sound! : (𝐄𝐅𝐐 ⊢! p) → (𝐈𝐧𝐭 W α) ⊧ p := λ ⟨d⟩ => sound d
+
+instance : Sound (𝐄𝐅𝐐 : AxiomSet α) (𝐈𝐧𝐭 W α) := ⟨sound!⟩
+
+end LO.Propositional.Superintuitionistic.Kripke
